CpcMini/SmtModel.lean
@@ -481,13 +481,7 @@ mutual
 
 def native_inhabited_type (T : SmtType) : native_Bool := by
   classical
-  exact
-    match T with
-    | SmtType.Datatype _ _ =>
-        native_and
-          (decide (__smtx_typeof_value (__smtx_type_default T) = T))
-          (__smtx_value_canonical_bool (__smtx_type_default T))
-    | _ => decide (∃ v : SmtValue, __smtx_typeof_value v = T)
+  exact decide (∃ v : SmtValue, __smtx_typeof_value v = T)
 
 def __vsm_apply_head : SmtValue -> SmtValue
   | (SmtValue.Apply f a) => (__vsm_apply_head f)
